function to remove conditions and TYPE args

HOL_To_IMP_Minus/Refinements/HOL_To_IMP_Minus_Datatypes.thy
@@ -1,8 +1,7 @@
 \<^marker>\<open>creator "Kevin Kappelmann"\<close>
 theory HOL_To_IMP_Minus_Datatypes
   imports
-    HOL_To_HOL_Nat.HOL_To_HOL_Nat_Basics
-    HOL_To_IMP_Minus_Primitives
+    HOL_To_IMP_Minus_Arithmetics
 begin
 
 locale HOL_To_HOL_Nat =
@@ -10,55 +9,49 @@ locale HOL_To_HOL_Nat =
   and transport_eq_restrict_id.partial_equivalence_rel_equivalence[per_intro del]
 begin
 
-case_of_simps append_eq_case : append.simps
-function_compile_nat append_eq_case
+paragraph \<open>rev\<close>
 
-case_of_simps rev_eq_case : rev.simps
-function_compile_nat rev_eq_case
+fun rev_aux :: "'a list \<Rightarrow> 'a list \<Rightarrow> 'a list" where
+  "rev_aux acc [] = acc" |
+  "rev_aux acc (x # xs) = rev_aux (x # acc) xs"
+
+case_of_simps rev_aux_eq : rev_aux.simps
+
+function_compile_nat rev_aux_eq
+
+definition rev :: "'a list \<Rightarrow> 'a list" where
+  "rev = rev_aux []"
+
+function_compile_nat rev_def
+
+paragraph \<open>zip\<close>
+
+thm zip.simps
+case_of_simps zip_eq : zip.simps
+function_compile_nat zip_eq
 
 end
+
+
 context HOL_To_IMP_Minus
 begin
 
-(*dummy stubs; need to compile fst_nat, snd_nat, pair_nat*)
-(*then we could compile constructors and automatically generated functions:*)
-thm Cons_nat_def
+compile_nat Cons_nat_def
+HOL_To_IMP_Minus_correct Cons_nat by cook
 
-declare_compiled_const fst_nat
-  return_register "fst.ret"
-  argument_registers "fst.args.x"
-  compiled suc_IMP
+compile_nat Nil_nat_def
+HOL_To_IMP_Minus_correct Nil_nat by cook
 
-declare_compiled_const snd_nat
-  return_register "fst.ret"
-  argument_registers "fst.args.x"
-  compiled suc_IMP
+thm HOL_To_HOL_Nat.rev_aux_nat_eq_unfolded
+lemmas rev_aux_nat_eq = HOL_To_HOL_Nat.rev_aux_nat_eq_unfolded[simplified case_list_nat_def]
+unconditional_nat rev_aux_nat_eq
+compile_nat rev_aux_nat_unconditional.simps
 
-declare_compiled_const Cons_nat
-  return_register "fst.ret"
-  argument_registers "fst.args.x" "fst.args.y"
-  compiled suc_IMP
-
-declare_compiled_const Pure.type
-  return_register "fst.ret"
-  argument_registers
-  compiled suc_IMP
-
-context
-  fixes xs' ys' :: "('a :: compile_nat) list"
-  assumes rels: "Rel_nat xs xs'" "Rel_nat xs ys'"
-begin
-
-lemmas test = HOL_To_HOL_Nat.append_nat_eq_unfolded[OF rels, unfolded case_list_nat_def]
-definition "blub x y \<equiv> HOL_To_HOL_Nat.append_nat TYPE('a) x y"
-
-lemma blub_rec: "blub x y =
-  (if fst_nat x = 0 then y else Cons_nat (fst_nat (snd_nat x)) (blub (snd_nat (snd_nat x)) y))"
-  unfolding blub_def by (subst test) (rule refl)
-
-compile_nat blub_rec
-
-end
+(*
+thm HOL_To_HOL_Nat.rev_nat_eq_unfolded
+lemmas rev_nat_eq = HOL_To_HOL_Nat.rev_nat_eq_unfolded[simplified case_list_nat_def]
+unconditional_nat rev_nat_eq
+*)
 
 end
 
